src/ExecuteI.v
@@ -37,104 +37,104 @@ Definition execute {p} {t} `{(RiscvState p t)}
     | Decode.Jal rd jimm20 =>
         Bind getPC (fun pc =>
                 let newPC := pc + fromImm jimm20 in
-                if (remu newPC four /= zero) : bool
-                then raiseException zero zero
-                else (Bind (setRegister rd (pc + four)) (fun _ => setPC newPC)))
+                if (remu newPC (ZToReg 4) /= ZToReg 0) : bool
+                then raiseException (ZToReg 0) (ZToReg 0)
+                else (Bind (setRegister rd (pc + ZToReg 4)) (fun _ => setPC newPC)))
     | Decode.Jalr rd rs1 oimm12 =>
         Bind (getRegister rs1) (fun x =>
                 Bind getPC (fun pc =>
-                        let newPC := and (x + fromImm oimm12) (lnot one) in
-                        if (remu newPC four /= zero) : bool
-                        then raiseException zero zero
-                        else (Bind (setRegister rd (pc + four)) (fun _ => setPC newPC))))
+                        let newPC := and (x + fromImm oimm12) (lnot (ZToReg 1)) in
+                        if (remu newPC (ZToReg 4) /= ZToReg 0) : bool
+                        then raiseException (ZToReg 0) (ZToReg 0)
+                        else (Bind (setRegister rd (pc + ZToReg 4)) (fun _ => setPC newPC))))
     | Decode.Beq rs1 rs2 sbimm12 =>
         Bind (getRegister rs1) (fun x =>
                 Bind (getRegister rs2) (fun y =>
                         Bind getPC (fun pc =>
                                 when (reg_eqb x y) (let newPC := (pc + fromImm sbimm12) in
-                                                    if (remu newPC four /= zero) : bool
-                                                    then raiseException zero zero
+                                                    if (remu newPC (ZToReg 4) /= ZToReg 0) : bool
+                                                    then raiseException (ZToReg 0) (ZToReg 0)
                                                     else setPC newPC))))
     | Decode.Bne rs1 rs2 sbimm12 =>
         Bind (getRegister rs1) (fun x =>
                 Bind (getRegister rs2) (fun y =>
                         Bind getPC (fun pc =>
                                 when (x /= y) (let addr := (pc + fromImm sbimm12) in
-                                               if (remu addr four /= zero) : bool
-                                               then raiseException zero zero
+                                               if (remu addr (ZToReg 4) /= ZToReg 0) : bool
+                                               then raiseException (ZToReg 0) (ZToReg 0)
                                                else setPC addr))))
     | Decode.Blt rs1 rs2 sbimm12 =>
         Bind (getRegister rs1) (fun x =>
                 Bind (getRegister rs2) (fun y =>
                         Bind getPC (fun pc =>
                                 when (x < y) (let addr := (pc + fromImm sbimm12) in
-                                              if (remu addr four /= zero) : bool
-                                              then raiseException zero zero
+                                              if (remu addr (ZToReg 4) /= ZToReg 0) : bool
+                                              then raiseException (ZToReg 0) (ZToReg 0)
                                               else setPC addr))))
     | Decode.Bge rs1 rs2 sbimm12 =>
         Bind (getRegister rs1) (fun x =>
                 Bind (getRegister rs2) (fun y =>
                         Bind getPC (fun pc =>
                                 when (x >= y) (let addr := (pc + fromImm sbimm12) in
-                                               if (remu addr four /= zero) : bool
-                                               then raiseException zero zero
+                                               if (remu addr (ZToReg 4) /= ZToReg 0) : bool
+                                               then raiseException (ZToReg 0) (ZToReg 0)
                                                else setPC addr))))
     | Decode.Bltu rs1 rs2 sbimm12 =>
         Bind (getRegister rs1) (fun x =>
                 Bind (getRegister rs2) (fun y =>
                         Bind getPC (fun pc =>
                                 when ((ltu x y)) (let addr := (pc + fromImm sbimm12) in
-                                                  if (remu addr four /= zero) : bool
-                                                  then raiseException zero zero
+                                                  if (remu addr (ZToReg 4) /= ZToReg 0) : bool
+                                                  then raiseException (ZToReg 0) (ZToReg 0)
                                                   else setPC addr))))
     | Decode.Bgeu rs1 rs2 sbimm12 =>
         Bind (getRegister rs1) (fun x =>
                 Bind (getRegister rs2) (fun y =>
                         Bind getPC (fun pc =>
                                 when (negb (ltu x y)) (let addr := (pc + fromImm sbimm12) in
-                                                       if (remu addr four /= zero) : bool
-                                                       then raiseException zero zero
+                                                       if (remu addr (ZToReg 4) /= ZToReg 0) : bool
+                                                       then raiseException (ZToReg 0) (ZToReg 0)
                                                        else setPC addr))))
     | Decode.Lb rd rs1 oimm12 =>
         Bind (getRegister rs1) (fun a =>
-                Bind (translate Load one (a + fromImm oimm12)) (fun addr =>
+                Bind (translate Load (ZToReg 1) (a + fromImm oimm12)) (fun addr =>
                         Bind (loadByte addr) (fun x => setRegister rd (int8ToReg x))))
     | Decode.Lh rd rs1 oimm12 =>
         Bind (getRegister rs1) (fun a =>
-                Bind (translate Load two (a + fromImm oimm12)) (fun addr =>
+                Bind (translate Load (ZToReg 2) (a + fromImm oimm12)) (fun addr =>
                         Bind (loadHalf addr) (fun x => setRegister rd (int16ToReg x))))
     | Decode.Lw rd rs1 oimm12 =>
         Bind (getRegister rs1) (fun a =>
-                Bind (translate Load four (a + fromImm oimm12)) (fun addr =>
+                Bind (translate Load (ZToReg 4) (a + fromImm oimm12)) (fun addr =>
                         Bind (loadWord addr) (fun x => setRegister rd (int32ToReg x))))
     | Decode.Lbu rd rs1 oimm12 =>
         Bind (getRegister rs1) (fun a =>
-                Bind (translate Load one (a + fromImm oimm12)) (fun addr =>
+                Bind (translate Load (ZToReg 1) (a + fromImm oimm12)) (fun addr =>
                         Bind (loadByte addr) (fun x => setRegister rd (uInt8ToReg x))))
     | Decode.Lhu rd rs1 oimm12 =>
         Bind (getRegister rs1) (fun a =>
-                Bind (translate Load two (a + fromImm oimm12)) (fun addr =>
+                Bind (translate Load (ZToReg 2) (a + fromImm oimm12)) (fun addr =>
                         Bind (loadHalf addr) (fun x => setRegister rd (uInt16ToReg x))))
     | Decode.Sb rs1 rs2 simm12 =>
         Bind (getRegister rs1) (fun a =>
-                Bind (translate Store one (a + fromImm simm12)) (fun addr =>
+                Bind (translate Store (ZToReg 1) (a + fromImm simm12)) (fun addr =>
                         Bind (getRegister rs2) (fun x => storeByte addr (regToInt8 x))))
     | Decode.Sh rs1 rs2 simm12 =>
         Bind (getRegister rs1) (fun a =>
-                Bind (translate Store two (a + fromImm simm12)) (fun addr =>
+                Bind (translate Store (ZToReg 2) (a + fromImm simm12)) (fun addr =>
                         Bind (getRegister rs2) (fun x => storeHalf addr (regToInt16 x))))
     | Decode.Sw rs1 rs2 simm12 =>
         Bind (getRegister rs1) (fun a =>
-                Bind (translate Store four (a + fromImm simm12)) (fun addr =>
+                Bind (translate Store (ZToReg 4) (a + fromImm simm12)) (fun addr =>
                         Bind (getRegister rs2) (fun x => storeWord addr (regToInt32 x))))
     | Decode.Addi rd rs1 imm12 =>
         Bind (getRegister rs1) (fun x => setRegister rd (x + fromImm imm12))
     | Decode.Slti rd rs1 imm12 =>
         Bind (getRegister rs1) (fun x =>
-                setRegister rd (if x < fromImm imm12 : bool then one else zero))
+                setRegister rd (if x < fromImm imm12 : bool then ZToReg 1 else ZToReg 0))
     | Decode.Sltiu rd rs1 imm12 =>
         Bind (getRegister rs1) (fun x =>
-                setRegister rd (if (ltu x (fromImm imm12)) : bool then one else zero))
+                setRegister rd (if (ltu x (fromImm imm12)) : bool then ZToReg 1 else ZToReg 0))
     | Decode.Xori rd rs1 imm12 =>
         Bind (getRegister rs1) (fun x => setRegister rd (xor x (fromImm imm12)))
     | Decode.Ori rd rs1 imm12 =>
@@ -159,11 +159,11 @@ Definition execute {p} {t} `{(RiscvState p t)}
     | Decode.Slt rd rs1 rs2 =>
         Bind (getRegister rs1) (fun x =>
                 Bind (getRegister rs2) (fun y =>
-                        setRegister rd (if x < y : bool then one else zero)))
+                        setRegister rd (if x < y : bool then ZToReg 1 else ZToReg 0)))
     | Decode.Sltu rd rs1 rs2 =>
         Bind (getRegister rs1) (fun x =>
                 Bind (getRegister rs2) (fun y =>
-                        setRegister rd (if (ltu x y) : bool then one else zero)))
+                        setRegister rd (if (ltu x y) : bool then ZToReg 1 else ZToReg 0)))
     | Decode.Xor rd rs1 rs2 =>
         Bind (getRegister rs1) (fun x =>
                 Bind (getRegister rs2) (fun y => setRegister rd (xor x y)))
@@ -185,16 +185,16 @@ Definition execute {p} {t} `{(RiscvState p t)}
     end.
 
 (* External variables:
-     Bind Load Return RiscvState Store and bool four fromImm getPC getRegister
-     int16ToReg int32ToReg int8ToReg lnot loadByte loadHalf loadWord ltu negb one
+     Bind Load Return RiscvState Store ZToReg and bool fromImm getPC getRegister
+     int16ToReg int32ToReg int8ToReg lnot loadByte loadHalf loadWord ltu negb
      op_zgze__ op_zl__ op_zm__ op_zp__ op_zsze__ or raiseException regToInt16
      regToInt32 regToInt8 regToShamt reg_eqb remu setPC setRegister sll sra srl
-     storeByte storeHalf storeWord translate tt two uInt16ToReg uInt8ToReg unit when
-     xor zero Decode.Add Decode.Addi Decode.And Decode.Andi Decode.Auipc Decode.Beq
-     Decode.Bge Decode.Bgeu Decode.Blt Decode.Bltu Decode.Bne Decode.Fence
-     Decode.Fence_i Decode.InstructionI Decode.Jal Decode.Jalr Decode.Lb Decode.Lbu
-     Decode.Lh Decode.Lhu Decode.Lui Decode.Lw Decode.Or Decode.Ori Decode.Sb
-     Decode.Sh Decode.Sll Decode.Slli Decode.Slt Decode.Slti Decode.Sltiu Decode.Sltu
+     storeByte storeHalf storeWord translate tt uInt16ToReg uInt8ToReg unit when xor
+     Decode.Add Decode.Addi Decode.And Decode.Andi Decode.Auipc Decode.Beq Decode.Bge
+     Decode.Bgeu Decode.Blt Decode.Bltu Decode.Bne Decode.Fence Decode.Fence_i
+     Decode.InstructionI Decode.Jal Decode.Jalr Decode.Lb Decode.Lbu Decode.Lh
+     Decode.Lhu Decode.Lui Decode.Lw Decode.Or Decode.Ori Decode.Sb Decode.Sh
+     Decode.Sll Decode.Slli Decode.Slt Decode.Slti Decode.Sltiu Decode.Sltu
      Decode.Sra Decode.Srai Decode.Srl Decode.Srli Decode.Sub Decode.Sw Decode.Xor
      Decode.Xori
 *)
