check_dep.sh
@@ -1,0 +1,16 @@
+#!/bin/sh
+
+if [ "$#" -ne 2 ]; then
+    echo "Usage: 2 args: directory of dependency to check and expected commit hash"
+    exit 1
+fi
+
+d=$1
+
+EXPECTED=$2
+ACTUAL=`cd $d && git rev-parse HEAD`
+if [ "$ACTUAL" != "$EXPECTED" ]; then
+    echo "Commit hash of $d does not match: Expected $EXPECTED, but got $ACTUAL"
+    exit 1
+fi
+
